WIP: defining all the rules for the relation

rupicola/io/Compilation.fst
@@ -24,7 +24,16 @@ let rec compile #g #a (#s:fs_oval g a) (qs:g ⊢ s) : Tot exp (decreases qs) =
   | QInl qp -> EInl (compile qp)
   | QInr qp -> EInr (compile qp)
   | QCase cond inlc inrc -> ECase (compile cond) (compile inlc) (compile inrc)
-  | _ -> admit ()
+  | QLambdaProd qbody -> ELam (compile_oprod qbody)
+and compile_oprod #g #a (#s:fs_oprod g a) (qs:oprod_quotation g s) : Tot exp (decreases qs) =
+  match qs with
+  | QRead -> ERead
+  | QWrite qarg -> EWrite (compile qarg)
+  | QReturn qx -> compile qx
+  | QBindProd qm qk -> EApp (ELam (compile_oprod qk)) (compile_oprod qm)
+  | QAppProd qf qx -> EApp (compile qf) (compile qx)
+  | QIfProd qc qt qe -> EIf (compile qc) (compile_oprod qt) (compile_oprod qe)
+  | QCaseProd qcond qinlc qinrc -> ECase (compile qcond) (compile_oprod qinlc) (compile_oprod qinrc)
 
 let lem_compile_empty_closed #a (#s:fs_oval empty a) (qs:empty ⊢ s) : Lemma (is_closed (compile qs)) = admit ()
 
@@ -45,14 +54,9 @@ let rec compile_equiv #g (#a:qType) (#s:fs_oval g a) (qs:g ⊢ s)
     compile_equiv qf;
     compile_equiv qx;
     equiv_app f x (compile qf) (compile qx)
-  | QLambda #_ #_ #_ #f qbody ->
+  | QLambda #_ #_ #_ #body qbody ->
     compile_equiv qbody;
-    equiv_lam f (compile qbody);
-    assert (s `equiv_oval a` (ELam (compile qbody)));
-    assert (s `equiv_oval a` (compile qs)) by (
-      norm [delta_only [`%compile]; zeta;iota];
-      rewrite_eqs_from_context ();
-      assumption ())
+    equiv_lam body (compile qbody)
   | QFalse -> equiv_false g
   | QTrue -> equiv_true g
   | QIf #_ #_ #c qc #t qt #e qe ->
@@ -81,7 +85,38 @@ let rec compile_equiv #g (#a:qType) (#s:fs_oval g a) (qs:g ⊢ s)
     compile_equiv qinlc;
     compile_equiv qinrc;
     equiv_case cond inlc inrc (compile qcond) (compile qinlc) (compile qinrc)
-  | _ -> admit ()
+  | QLambdaProd #_ #_ #_ #body qbody ->
+    compile_equiv_prod qbody;
+    equiv_lam_prod body (compile_oprod qbody)
+and compile_equiv_prod #g (#a:qType) (#s:fs_oprod g a) (qs:oprod_quotation g s)
+  : Lemma (ensures (s `equiv_oprod a` (compile_oprod qs))) (decreases qs)
+  =
+  match qs with
+  | QRead -> equiv_oprod_read g
+  | QWrite #_ #arg qarg ->
+    compile_equiv qarg;
+    equiv_oprod_write arg (compile qarg)
+  | QReturn #_ #_ #x qx ->
+    compile_equiv qx;
+    equiv_oprod_return x (compile qx)
+  | QBindProd #_ #_ #_ #m #k qm qk ->
+    compile_equiv_prod qm;
+    compile_equiv_prod qk;
+    equiv_oprod_bind m k (compile_oprod qm) (compile_oprod qk)
+  | QAppProd #_ #_ #_ #f #x qf qx ->
+    compile_equiv qf;
+    compile_equiv qx;
+    equiv_oprod_app f x (compile qf) (compile qx)
+  | QIfProd #_ #_ #c qc #t qt #e qe ->
+    compile_equiv qc;
+    compile_equiv_prod qt;
+    compile_equiv_prod qe;
+    equiv_oprod_if c t e (compile qc) (compile_oprod qt) (compile_oprod qe)
+  | QCaseProd #_ #_ #_ #_ #cond qcond #inlc qinlc #inrc qinrc ->
+    compile_equiv qcond;
+    compile_equiv_prod qinlc;
+    compile_equiv_prod qinrc;
+    equiv_oprod_case cond inlc inrc (compile qcond) (compile_oprod qinlc) (compile_oprod qinrc)
 
 let compile_closed_equiv (#a:qType) (#s:get_Type a) (qs: a ⊩ s)
   : Lemma (ensures (forall h. a ⦂ (h, s, compile_closed qs))) =
